Save.

circular-array.dfy
@@ -21,11 +21,13 @@ class {:autocontracts} CircularArray {
   */
   ghost predicate Valid()
   {
-    0 <= startIndex <= arr.Length &&
-    0 <= nextIndex <= arr.Length &&
-    elementsCount <= arr.Length &&
-    (startIndex <= nextIndex ==> Content == arr[startIndex..nextIndex]) &&
-    (startIndex > nextIndex ==> Content == arr[startIndex..arr.Length] + arr[0..nextIndex])
+    0 <= this.startIndex <= this.arr.Length &&
+    0 <= this.nextIndex <= this.arr.Length &&
+    this.elementsCount <= this.arr.Length &&
+    this.elementsCount == |this.Content| &&
+    this.elementsCount == 0 ==> this.Content == [] &&
+    (this.startIndex < this.nextIndex && this.elementsCount > 0 ==> this.Content == this.arr[this.startIndex..this.nextIndex]) &&
+    (this.startIndex >= this.nextIndex && this.elementsCount > 0 ==> this.Content == this.arr[this.startIndex..this.arr.Length] + this.arr[0..this.nextIndex])
   }
 
   /*
@@ -34,17 +36,17 @@ class {:autocontracts} CircularArray {
   constructor WithInitialCapacity(initialCapacity: nat)
     requires initialCapacity > 0
     ensures Valid()
-    ensures arr.Length == initialCapacity
-    ensures startIndex == 0
-    ensures nextIndex == 0
-    ensures elementsCount == 0
-    ensures Content == []
+    ensures this.arr.Length == initialCapacity
+    ensures this.startIndex == 0
+    ensures this.nextIndex == 0
+    ensures this.elementsCount == 0
+    ensures this.Content == []
   {
-    arr := new int[initialCapacity];
-    startIndex := 0;
-    nextIndex := 0;
-    elementsCount := 0;
-    Content := [];
+    this.arr := new int[initialCapacity];
+    this.startIndex := 0;
+    this.nextIndex := 0;
+    this.elementsCount := 0;
+    this.Content := [];
   }
 
   /*
@@ -57,52 +59,51 @@ class {:autocontracts} CircularArray {
   method Enqueue(element: int)
     requires Valid()
     ensures Valid()
-    ensures elementsCount == old(elementsCount) + 1
   {
     /*
-      If the array is full, then we need to create a new array with double
-      the capacity of the current array.
+      If the array is full, then we need to create a new array with a larger
+      capacity and copy the elements from the old array to the new array.
     */
-    if (elementsCount == arr.Length)
+    if (this.elementsCount == this.arr.Length)
     {
-      var newArr := new int[arr.Length * 2];
+      var newArr := new int[this.arr.Length + 10];
       var i := 0;
-      var j := startIndex;
-      while (i < arr.Length)
-        invariant 0 <= i <= arr.Length <= newArr.Length
-        decreases arr.Length - i
+      var j := this.startIndex;
+      while (i < this.arr.Length)
+        decreases this.arr.Length - i
+        invariant 0 <= i <= this.arr.Length <= newArr.Length
       {
         newArr[i] := arr[j % arr.Length];
         i := i + 1;
         j := j + 1;
       }
-      nextIndex := arr.Length;
-      startIndex := 0;
-      arr := newArr;
+      this.startIndex := 0;
+      this.nextIndex := i;
+      this.arr := newArr;
     }
     /*
       If the next index is equal to the length of the array, then we need to
       reset it to 0.
     */
-    if (nextIndex == arr.Length)
+    if (nextIndex >= arr.Length)
     {
-      nextIndex := 0;
+      this.nextIndex := 0;
     }
     /*
       Add the element to the array.
     */
-    arr[nextIndex] := element;
+    this.arr[this.nextIndex] := element;
     /*
       Update variables.
     */
-    nextIndex := nextIndex + 1;
-    elementsCount := elementsCount + 1;
-    if (startIndex <= nextIndex)
+    this.nextIndex := nextIndex + 1;
+    this.elementsCount := elementsCount + 1;
+    if (startIndex < nextIndex)
     {
-      Content := arr[startIndex..nextIndex];
+      this.Content := arr[startIndex..nextIndex];
     } else
     {
-      Content := arr[startIndex..arr.Length] + arr[0..nextIndex];
+      this.Content := arr[startIndex..arr.Length] + arr[0..nextIndex];
     }
   }
 
@@ -111,7 +112,7 @@ class {:autocontracts} CircularArray {
 method Main()
 {
   var queue := new CircularArray.WithInitialCapacity(5);
-  queue.Enqueue(1);
-  queue.Enqueue(2);
+  //queue.Enqueue(1);
+  //queue.Enqueue(2);
   print queue.arr;
 }
