circular-array-2.dfy
@@ -1,0 +1,74 @@
+/*
+  Class CircularArray.
+*/
+class {:autocontracts} CircularArray {
+    /*
+      Implementation
+    */
+    var a: array<int>; // The array.
+    var startIndex: nat; // The index of the first element.
+    var currentIndex: nat; // The index to put the next element.
+    var count: nat; // The number of elements.
+
+    /*
+      Abstraction.
+    */
+    ghost var Elements: seq<int>; // The elements in the array represented as a sequence.
+
+    /*
+      Class invariant.
+    */
+    ghost predicate Valid()
+    {
+        0 <= startIndex <= a.Length &&
+        0 <= currentIndex <= a.Length &&
+        0 <= count <= a.Length &&
+        count == |Elements| &&
+        forall i: nat :: 0 <= i < count ==> Elements[i] == a[(startIndex + i) % a.Length]
+    }
+
+    /*
+      Constructor.
+    */
+    constructor WithInitialCapacity(capacity: nat)
+        requires capacity > 0
+        ensures Valid()
+    {
+        a := new int[capacity];
+        startIndex := 0;
+        currentIndex := 0;
+        count := 0;
+        Elements := [];
+    }
+
+    /*
+      Contains method.
+    */
+    method Contains(element: int) returns (r: bool)
+        requires Valid()
+        ensures Valid()
+        ensures r == (element in Elements)
+    {
+        r := false;
+        var i := 0;
+        while i < count
+            invariant 0 <= i <= count
+            invariant r == (element in Elements[0..i])
+            decreases count - i
+        {
+            if (a[(startIndex + i) % a.Length] == element) {
+                r := true;
+            }
+            i := i + 1;
+        }
+    }
+
+    /*
+        Size function.
+    */
+    function Size(): nat
+        ensures Size() == count
+    {
+        count
+    }
+}
