test.dfy
@@ -1,0 +1,21 @@
+method Main()
+{
+    var a := new int[5];
+    a[0] := 1;
+    a[1] := 2;
+    a[2] := 3;
+    a[3] := 4;
+    a[4] := 5;
+    var startIndex := 0;
+    var endIndex := 0;
+    var s:seq<int> := [];
+    if (startIndex < endIndex)
+    {
+        s := a[startIndex..endIndex];
+    } else {
+        s := a[startIndex..a.Length] + a[0..endIndex];
+    }
+    print s;
+    var d := [1,2,3];
+    print d[0..2];
+}
